Finish if_case equivalence example

src/FrameStack/Examples.v
@@ -27,6 +27,7 @@ Ltac deriv :=
   | [H : | _ :: _, RExc _ | _ ↓ |- _] => inv H; try inv_val
   | [H : | _, RExp (EExp _) | _ ↓ |- _] => inv H; try inv_val
   | [H : | _, RExp (VVal _) | _ ↓ |- _] => inv H; try inv_val
+  | [H : | _, RBox | _ ↓ |- _] => inv H; try inv_val
   end.
 
 Ltac extract_meta_eval H :=
@@ -73,19 +74,21 @@ Section case_if_equiv.
     ELet 1 e1
       (ECase (`VVar 0) 
               [([PLit (Atom "true")], `VLit "true", e2);
-              ([PVar], `VLit "true", e3)]).
+              ([PVar], `VLit "true", e3.[ren (fun n => 2 + n) ])]).
 
   Local Definition idiomatic :=
     ELet 1 e1
       (ECase (EValues [])
-          [([], °ECall "=:=" [`VVar 0;`VLit "true"], e2);
-          ([], `VLit "true", e3)]).
+          [([], °ECall "erlang" "=:=" [`VVar 0;`VLit "true"], e2);
+          ([], `VLit "true", e3.[ren (fun n => 1 + n) ])]).
 
   Local Proposition nonidiomatic_scope :
     EXP Γ ⊢ nonidiomatic.
   Proof.
     unfold nonidiomatic.
     scope_solver.
+    apply -> subst_preserves_scope_exp. exact He3.
+    intro. intros. simpl. lia. 
   Qed.
 
   Local Proposition idiomatic_scope :
@@ -93,9 +96,11 @@ Section case_if_equiv.
   Proof.
     unfold idiomatic.
     scope_solver.
+    apply -> subst_preserves_scope_exp. exact He3.
+    intro. intros. simpl. lia. 
   Qed.
 
-  Local Theorem equivalence :
+  Local Theorem equivalence_part1 :
     CIU_open Γ nonidiomatic idiomatic.
   Proof.
     split. 2: split.
@@ -122,30 +127,118 @@ Section case_if_equiv.
           break_match_hyp; try congruence. destruct l; simpl in Heqb; try congruence.
           break_match_hyp; try congruence. inv Heqo. simpl in H10. inv H10.
           simpl in H11. do 2 deriv.
+          cbn in H9. inv H9.
           unfold idiomatic.
-          exists (S (15 + k2 + k0)). simpl. econstructor.
+          exists (S (12 + k2 + k0)). simpl. econstructor.
           eapply frame_indep_nil in Hd.
           eapply step_term_term. eassumption. 2: lia.
-          replace counter with (15 + k2).
+          replace counter with (12 + k2).
+          constructor. reflexivity.
+          simpl. constructor.
+          constructor. econstructor. congruence. simpl. reflexivity.
+          econstructor. reflexivity.
+          simpl. constructor. econstructor. congruence.
+          constructor. constructor. constructor. simpl. econstructor. cbn. reflexivity.
+          econstructor. reflexivity. eassumption.
+        }
+        { (* v is not true *)
+          deriv.
+          2: { (* no more cases *)
+            inv H9.
+          }
+          simpl in H12. do 2 deriv. rewrite H11 in H9. inv H9.
+          unfold idiomatic.
+          exists (S (15 + k1 + k0)). simpl. econstructor.
+          eapply frame_indep_nil in Hd.
+          eapply step_term_term. eassumption. 2: lia.
+          replace counter with (15 + k1).
           constructor. reflexivity.
           simpl. constructor.
           constructor. econstructor. congruence. simpl. reflexivity.
           econstructor. reflexivity.
           simpl. constructor. econstructor. congruence.
           constructor. constructor. constructor. simpl. econstructor.
-          unfold create_result.
+          { (* v is not true *)
+            cbn. clear Hd H11 H12 H6. destruct v; simpl; try reflexivity.
+            2: destruct n; reflexivity.
+            destruct l; try reflexivity. simpl.
+            destruct string_dec; try reflexivity. subst. simpl in H10. congruence.
+          } 
+          constructor. econstructor. reflexivity. constructor. econstructor.
+          reflexivity.
+          simpl in H11. inv H11.
+          do 2 rewrite subst_comp_exp in *.
+          clear Hd H10. cbn in *.
+          rewrite substcomp_id_r.
+          rewrite subst_extend in H12.
+          rewrite substcomp_scons_core, subst_extend in H12.
+          rewrite subst_extend.
+          rewrite subst_comp_exp in *.
+          rewrite ren_scons in *.
+          rewrite ren_scons in H12. assumption.
         }
-        { (* v is not true *)
-
-        }
-        
       }
     }
   Qed.
-  Local Theorem equivalence :
-    CIU idiomatic nonidiomatic.
-  Proof.
 
+  Local Theorem equivalence_part2 :
+    CIU_open Γ idiomatic nonidiomatic.
+  Proof.
+    apply Rrel_implies_CIU.
+    apply Rrel_exp_compat. apply Erel_Let_compat; auto.
+    apply Rrel_exp_compat_reverse. apply CIU_implies_Rrel.
+    pose proof (nonidiomatic_scope).
+    pose proof (idiomatic_scope).
+    unfold idiomatic, nonidiomatic in *. inv H. inv H0. inv H3. inv H2.
+    split. 2: split.
+    1-2: constructor; apply -> subst_preserves_scope_exp; eauto.
+    clear H6 H3 H7. intros. simpl in H1.
+    do 4 deriv. simpl in H9. deriv. 2: { inv H11. }
+    inv H11.
+    simpl in H12. rewrite idsubst_is_id_val in H12. do 3 deriv.
+    break_match_hyp.
+    2: { (* technical, Q: should this be possible? Evaluation of variables shouldn't just fail? -> variables are values or expressions? *)
+      do 3 deriv. cbn in H11.
+      do 2 deriv. 2: { deriv. inv H12. }
+      simpl in H13. do 2 deriv. inv H11. inv H12.
+      exists (6 + k0). simpl.
+      econstructor. rewrite Heqs. do 2 constructor. reflexivity.
+      econstructor. reflexivity. simpl. constructor. econstructor.
+      reflexivity. simpl.
+      rewrite subst_comp_exp in *. simpl in *.
+      rewrite subst_extend, subst_comp_exp in *.
+      rewrite substcomp_id_r, ren_scons in *. assumption.
+    }
+    do 3 deriv. cbn in H11.
+    break_match_hyp.
+    { (* e1 is true *)
+      deriv. inv H9. simpl in H12. rewrite idsubst_is_id_exp in H12.
+      exists (5 + k). simpl.
+      econstructor. rewrite Heqs.
+      destruct v; simpl in Heqb; try congruence.
+      destruct l; simpl in Heqb; try congruence.
+      break_match_hyp; try congruence. subst.
+      econstructor. econstructor. reflexivity.
+      constructor. econstructor. reflexivity.
+      simpl. now rewrite idsubst_is_id_exp.
+    }
+    { (* e1 is false *)
+      do 2 deriv. 2: { inv H12. }
+      simpl in H13. do 2 deriv. inv H12. inv H11.
+      exists (6 + k0). simpl.
+      econstructor. rewrite Heqs. do 2 constructor.
+      {
+        destruct v; simpl in Heqb; try reflexivity.
+        destruct l; simpl in Heqb; try reflexivity.
+        break_match_hyp; subst; try congruence.
+        cbn. destruct string_dec; auto. congruence.
+      }
+      econstructor. reflexivity. simpl. constructor. econstructor.
+      reflexivity. simpl.
+      rewrite subst_comp_exp in *. simpl in *.
+      rewrite subst_extend, subst_comp_exp in *.
+      rewrite substcomp_id_r, ren_scons in *. assumption.
+    }
   Qed.
 End case_if_equiv.
 
